projection/proofs/payload_to_cakemlProofScript.sml
@@ -8,80 +8,80 @@ open preamble
 val _ = new_theory "payload_to_cakemlProof";
 
 val has_v_def = Define
-  `has_v env n cfty f =
-   (?v. nsLookup env n = SOME v
-        /\ cfty f v)
-  `
+  ‘has_v env n cfty f =
+   (∃v. nsLookup env n = SOME v
+        ∧ cfty f v)
+  ’;
 
-val WORD8 = ``WORD:word8 -> v -> bool``
+val WORD8 = “WORD:word8 -> v -> bool”;
 
-val in_module_def = Define `
+val in_module_def = Define ‘
   in_module name =
-  !x y (env:(modN,varN,v) namespace). nsLookup (nsBind x y env) name = nsLookup env name
-  `;
+  ∀x y (env:(modN,varN,v) namespace). nsLookup (nsBind x y env) name = nsLookup env name
+  ’;
 
-val env_asm_def = Define `
+val env_asm_def = Define ‘
   env_asm env conf = (
-    has_v env.v conf.length (LIST_TYPE ^WORD8 --> NUM) LENGTH /\
-    has_v env.v conf.null (LIST_TYPE ^WORD8 --> BOOL) NULL /\
-    has_v env.v conf.take (LIST_TYPE ^WORD8 --> NUM --> LIST_TYPE ^WORD8) (combin$C TAKE) /\
-    has_v env.v conf.drop (LIST_TYPE ^WORD8 --> NUM --> LIST_TYPE ^WORD8) (combin$C DROP) /\
-    (?v. nsLookup env.v conf.fromList = SOME v /\
-         (!l lv.
+    has_v env.v conf.length (LIST_TYPE ^WORD8 --> NUM) LENGTH ∧
+    has_v env.v conf.null (LIST_TYPE ^WORD8 --> BOOL) NULL ∧
+    has_v env.v conf.take (LIST_TYPE ^WORD8 --> NUM --> LIST_TYPE ^WORD8) (combin$C TAKE) ∧
+    has_v env.v conf.drop (LIST_TYPE ^WORD8 --> NUM --> LIST_TYPE ^WORD8) (combin$C DROP) ∧
+    (∃v. nsLookup env.v conf.fromList = SOME v ∧
+         (∀l lv.
            LIST_TYPE ^WORD8 l lv
-           ==> !s1: unit semanticPrimitives$state. ?env' exp ck1 ck2. do_opapp [v; lv] = SOME(env',exp)
-               /\ evaluate (s1 with clock := ck1) env' [exp] =
-                  (s1 with <|clock := ck2; refs := s1.refs ++ [W8array l]|>,Rval [Loc(LENGTH s1.refs)]))) /\
-    in_module conf.length /\
-    in_module conf.null /\
-    in_module conf.take /\
-    in_module conf.drop /\
+           ⇒ ∀s1: unit semanticPrimitives$state. ∃env' exp ck1 ck2. do_opapp [v; lv] = SOME(env',exp)
+               ∧ evaluate (s1 with clock := ck1) env' [exp] =
+                  (s1 with <|clock := ck2; refs := s1.refs ++ [W8array l]|>,Rval [Loc(LENGTH s1.refs)]))) ∧
+    in_module conf.length ∧
+    in_module conf.null ∧
+    in_module conf.take ∧
+    in_module conf.drop ∧
     in_module conf.fromList)
-  `;
+  ’;
 
 
 val evaluate_empty_state_norel = Q.prove(
-  `∀s x refs refs' exp env ck1 ck2.
+  ‘∀s x refs refs' exp env ck1 ck2.
     evaluate (empty_state with <|clock := ck1; refs := refs|>) env [exp] =
              (empty_state with <|clock := ck2; refs := refs ++ refs'|>,Rval [x]) ⇒
     ∃ck1 ck2.
       evaluate (s with <|clock := ck1; refs := refs; ffi:= s.ffi|>) env [exp] =
-      (s with <|clock := ck2; refs := refs ++ refs'; ffi:= s.ffi|>,Rval [x])`,
+      (s with <|clock := ck2; refs := refs ++ refs'; ffi:= s.ffi|>,Rval [x])’,
   rpt strip_tac >>
-  qabbrev_tac `a1 = s with refs := refs` >>
-  `refs = a1.refs` by(qunabbrev_tac `a1` >> simp[]) >>
+  qabbrev_tac ‘a1 = s with refs := refs’ >>
+  ‘refs = a1.refs’ by(qunabbrev_tac ‘a1’ >> simp[]) >>
   fs[] >>
   drule (SIMP_RULE (srw_ss()) [ml_progTheory.eval_rel_def,PULL_EXISTS] evaluate_empty_state_IMP
          |> GEN_ALL) >>
   unabbrev_all_tac >>
-  Cases_on `s` >> fs[state_fn_updates]);
+  Cases_on ‘s’ >> fs[state_fn_updates]);
 
-val LUPDATE_REPLICATE = Q.store_thm("LUPDATE_REPLICATE",
-  `!n m x y. n < m ==>
-   LUPDATE x n (REPLICATE m y) = REPLICATE n y ++ [x] ++ REPLICATE (m - (n + 1)) y`,
-  Induct >> Cases >> rw[LUPDATE_def] >> simp[ADD1]);
+Theorem LUPDATE_REPLICATE
+  ‘∀n m x y. n < m ⇒
+   LUPDATE x n (REPLICATE m y) = REPLICATE n y ++ [x] ++ REPLICATE (m - (n + 1)) y’
+ (Induct >> Cases >> rw[LUPDATE_def] >> simp[ADD1]);
 
-val padv_correct = Q.store_thm("padv_correct",`
-  !env conf l lv le s1 s2 refs.
-  env_asm env conf /\
-  LIST_TYPE ^WORD8 l lv /\
+Theorem padv_correct
+ ‘∀env conf l lv le s1 s2 refs.
+  env_asm env conf ∧
+  LIST_TYPE ^WORD8 l lv ∧
   evaluate$evaluate s1 env [le] = (s2 with refs := s1.refs ++ refs, Rval [lv])
-  ==>
-  ?ck1 ck2 refs' num lv'.
+  ⇒
+  ∃ck1 ck2 refs' num lv'.
   evaluate$evaluate (s1 with clock:= ck1) env [App Opapp [padv conf; le]] =
-           (s2 with <|clock := ck2; refs := APPEND s1.refs refs'|>, Rval [Loc num]) /\
+           (s2 with <|clock := ck2; refs := APPEND s1.refs refs'|>, Rval [Loc num]) ∧
   store_lookup num (APPEND s1.refs refs') = SOME(W8array(pad conf l))
-  `,
-  rpt strip_tac >>
+  ’
+ (rpt strip_tac >>
   drule evaluate_add_to_clock >>
   simp[] >>
-  qabbrev_tac `ack = s2.clock` >>
+  qabbrev_tac ‘ack = s2.clock’ >>
   fs[env_asm_def,in_module_def,has_v_def] >>
   strip_tac >>
-  Q.REFINE_EXISTS_TAC `extra + s1.clock` >>
+  Q.REFINE_EXISTS_TAC ‘extra + s1.clock’ >>
   simp[Once evaluate_def] >>
   simp[padv_def,do_opapp_def,buffer_size_def,payload_size_def] >>
-  Q.REFINE_EXISTS_TAC `extra + 1` >>
+  Q.REFINE_EXISTS_TAC ‘extra + 1’ >>
   simp[Once evaluate_def] >>
   simp[dec_clock_def,do_app_def,store_alloc_def,ml_progTheory.nsLookup_nsBind_compute,
        namespaceTheory.nsOptBind_def] >>
@@ -91,20 +91,21 @@ val padv_correct = Q.store_thm("padv_correct",`
   ntac 6 (simp[Once evaluate_def]) >>
   simp[ml_progTheory.nsLookup_nsBind_compute] >>
   ntac 2 (simp[Once evaluate_def]) >>
-  qpat_assum `(LIST_TYPE ^WORD8 --> NUM) LENGTH _` (mp_tac o REWRITE_RULE[ml_translatorTheory.Arrow_def,ml_translatorTheory.AppReturns_def,ml_progTheory.eval_rel_def]) >>
-  simp[] >> disch_then drule >>
-  qmatch_goalsub_abbrev_tac `refs_fupd (K a1)` >>
-  disch_then(qspec_then `a1` strip_assume_tac) >>
-  qunabbrev_tac `a1` >>
-  Q.REFINE_EXISTS_TAC `extra + 1` >>
+  qpat_assum ‘(LIST_TYPE ^WORD8 --> NUM) LENGTH _’ (mp_tac o REWRITE_RULE[ml_translatorTheory.Arrow_def,ml_translatorTheory.AppReturns_def,ml_progTheory.eval_rel_def]) >>
+  simp[] >>
+  disch_then drule >>
+  qmatch_goalsub_abbrev_tac ‘refs_fupd (K a1)’ >>
+  disch_then(qspec_then ‘a1’ strip_assume_tac) >>
+  qunabbrev_tac ‘a1’ >>
+  Q.REFINE_EXISTS_TAC ‘extra + 1’ >>
   simp[dec_clock_def] >>
-  Q.ISPEC_THEN `s2 with refs := s1.refs ++ refs` dxrule evaluate_empty_state_norel >>
+  Q.ISPEC_THEN ‘s2 with refs := s1.refs ++ refs’ dxrule evaluate_empty_state_norel >>
   strip_tac >>
-  qmatch_asmsub_abbrev_tac `clock_fupd (K ack1)` >>
-  Q.REFINE_EXISTS_TAC `extra + ack1` >>
+  qmatch_asmsub_abbrev_tac ‘clock_fupd (K ack1)’ >>
+  Q.REFINE_EXISTS_TAC ‘extra + ack1’ >>
   drule evaluate_add_to_clock >>
-  simp[SimpL ``$==>``] >>
-  disch_then(qspec_then `ack` mp_tac) >>
+  simp[SimpL “$==>”] >>
+  disch_then(qspec_then ‘ack’ mp_tac) >>
   strip_tac >>
   dxrule evaluate_add_to_clock >>
   simp[] >>
@@ -113,83 +114,83 @@ val padv_correct = Q.store_thm("padv_correct",`
   simp[do_app_def] >>
   simp[terminationTheory.do_eq_def,lit_same_type_def,Boolv_def,do_if_def] >>
   PURE_REWRITE_TAC [ADD_ASSOC] >>
-  qpat_abbrev_tac `ack2 = ack + _` >> pop_assum kall_tac >>
-  Cases_on `LENGTH l = conf.payload_size` >-
+  qpat_abbrev_tac ‘ack2 = ack + _’ >> pop_assum kall_tac >>
+  Cases_on ‘LENGTH l = conf.payload_size’ >-
     (ntac 7 (simp[Once evaluate_def]) >>
      simp[do_app_def,store_lookup_def,EL_APPEND_EQN,store_assign_def,
           store_v_same_type_def,ml_progTheory.nsLookup_nsBind_compute,
           namespaceTheory.nsOptBind_def,lupdate_append2] >>
      ntac 10 (simp[Once evaluate_def]) >>
-     qpat_assum `(LIST_TYPE WORD --> NUM --> LIST_TYPE WORD) (combin$C TAKE) _` (mp_tac o REWRITE_RULE[ml_translatorTheory.Arrow_def,ml_translatorTheory.AppReturns_def,ml_progTheory.eval_rel_def]) >>
+     qpat_assum ‘(LIST_TYPE WORD --> NUM --> LIST_TYPE WORD) (combin$C TAKE) _’ (mp_tac o REWRITE_RULE[ml_translatorTheory.Arrow_def,ml_translatorTheory.AppReturns_def,ml_progTheory.eval_rel_def]) >>
      simp[] >> disch_then drule >>
-     qmatch_goalsub_abbrev_tac `refs_fupd (K a1)` >>     
-     disch_then(qspec_then `a1` strip_assume_tac) >>
-     qunabbrev_tac `a1` >>
-     Q.REFINE_EXISTS_TAC `extra + 1` >>
+     qmatch_goalsub_abbrev_tac ‘refs_fupd (K a1)’ >>     
+     disch_then(qspec_then ‘a1’ strip_assume_tac) >>
+     qunabbrev_tac ‘a1’ >> 
+     Q.REFINE_EXISTS_TAC ‘extra + 1’ >> 
      simp[dec_clock_def] >>
-     Q.ISPEC_THEN `s2 with refs := s1.refs ++ refs` dxrule evaluate_empty_state_norel >>
+     Q.ISPEC_THEN ‘s2 with refs := s1.refs ++ refs’ dxrule evaluate_empty_state_norel >>
      strip_tac >>
-     qmatch_asmsub_abbrev_tac `clock_fupd (K ack3)` >>
-     Q.REFINE_EXISTS_TAC `extra + ack3` >>
+     qmatch_asmsub_abbrev_tac ‘clock_fupd (K ack3)’ >>
+     Q.REFINE_EXISTS_TAC ‘extra + ack3’ >>
      drule evaluate_add_to_clock >>
-     simp[SimpL ``$==>``] >>
-     disch_then(qspec_then `ack2` mp_tac) >>
+     simp[SimpL “$==>”] >>
+     disch_then(qspec_then ‘ack2’ mp_tac) >>
      strip_tac >>
      dxrule evaluate_add_to_clock >>
      simp[] >> disch_then kall_tac >>
-     first_x_assum(qspecl_then [`conf.payload_size`,`Litv (IntLit (&conf.payload_size))`] mp_tac) >>
+     first_x_assum(qspecl_then [‘conf.payload_size’,‘Litv (IntLit (&conf.payload_size))’] mp_tac) >>
      impl_tac >- simp[NUM_def,INT_def] >>
-     qmatch_goalsub_abbrev_tac `refs_fupd (K a1)` >>
-     disch_then(qspec_then `a1` strip_assume_tac) >>
-     qunabbrev_tac `a1` >>
-     Q.REFINE_EXISTS_TAC `extra + 1` >>
+     qmatch_goalsub_abbrev_tac ‘refs_fupd (K a1)’ >>
+     disch_then(qspec_then ‘a1’ strip_assume_tac) >>
+     qunabbrev_tac ‘a1’ >>
+     Q.REFINE_EXISTS_TAC ‘extra + 1’ >>
      simp[dec_clock_def] >>
      PURE_REWRITE_TAC [ADD_ASSOC] >>
-     qpat_abbrev_tac `ack4 = ack2 + _` >> pop_assum kall_tac >>
-     Q.ISPEC_THEN `s2 with refs := s1.refs ++ refs` dxrule evaluate_empty_state_norel >>
+     qpat_abbrev_tac ‘ack4 = ack2 + _’ >> pop_assum kall_tac >>
+     Q.ISPEC_THEN ‘s2 with refs := s1.refs ++ refs’ dxrule evaluate_empty_state_norel >>
      strip_tac >>
-     qmatch_asmsub_abbrev_tac `clock_fupd (K ack5)` >>
-     Q.REFINE_EXISTS_TAC `extra + ack5` >>
+     qmatch_asmsub_abbrev_tac ‘clock_fupd (K ack5)’ >>
+     Q.REFINE_EXISTS_TAC ‘extra + ack5’ >>
      drule evaluate_add_to_clock >>
-     simp[SimpL ``$==>``] >>
-     disch_then(qspec_then `ack4` mp_tac) >>
+     simp[SimpL “$==>”] >>
+     disch_then(qspec_then ‘ack4’ mp_tac) >>
      strip_tac >>
      dxrule evaluate_add_to_clock >>
      simp[] >>
      disch_then kall_tac >>
      PURE_REWRITE_TAC [ADD_ASSOC] >>
-     qpat_abbrev_tac `ack6 = ack4 + _` >> pop_assum kall_tac >>
+     qpat_abbrev_tac ‘ack6 = ack4 + _’ >> pop_assum kall_tac >>
      simp[Once evaluate_def] >>
      last_x_assum drule >>
-     qmatch_goalsub_abbrev_tac `refs_fupd (K a1)` >>
-     disch_then(qspec_then `empty_state with refs := a1` mp_tac) >>
+     qmatch_goalsub_abbrev_tac ‘refs_fupd (K a1)’ >>
+     disch_then(qspec_then ‘empty_state with refs := a1’ mp_tac) >>
      simp[] >>
-     qunabbrev_tac `a1` >> strip_tac >>
-     Q.REFINE_EXISTS_TAC `extra + 1` >>
+     qunabbrev_tac ‘a1’ >> strip_tac >>
+     Q.REFINE_EXISTS_TAC ‘extra + 1’ >>
      simp[dec_clock_def] >>
-     Q.ISPEC_THEN `s2 with refs := s1.refs ++ refs` dxrule evaluate_empty_state_norel >>
+     Q.ISPEC_THEN ‘s2 with refs := s1.refs ++ refs’ dxrule evaluate_empty_state_norel >>
      strip_tac >>
-     qmatch_asmsub_abbrev_tac `clock_fupd (K ack7)` >>
-     Q.REFINE_EXISTS_TAC `extra + ack7` >>
+     qmatch_asmsub_abbrev_tac ‘clock_fupd (K ack7)’ >>
+     Q.REFINE_EXISTS_TAC ‘extra + ack7’ >>
      drule evaluate_add_to_clock >>
-     simp[SimpL ``$==>``] >>
-     disch_then(qspec_then `ack6` mp_tac) >>
+     simp[SimpL “$==>”] >>
+     disch_then(qspec_then ‘ack6’ mp_tac) >>
      strip_tac >>
      dxrule evaluate_add_to_clock >>
      simp[] >> disch_then kall_tac >>
      PURE_REWRITE_TAC [ADD_ASSOC] >>
-     qpat_abbrev_tac `ack8 = ack6 + _` >> pop_assum kall_tac >>
+     qpat_abbrev_tac ‘ack8 = ack6 + _’ >> pop_assum kall_tac >>
      simp[evaluate_def,namespaceTheory.nsOptBind_def,ml_progTheory.nsLookup_nsBind_compute,
           do_app_def,store_lookup_def,EL_APPEND_EQN,copy_array_def,integerTheory.INT_ABS,
           LUPDATE_APPEND,LUPDATE_def] >>
-     qmatch_goalsub_abbrev_tac `lhs < rhs` >>
-    `rhs = lhs`
+     qmatch_goalsub_abbrev_tac ‘lhs < rhs’ >>
+    ‘rhs = lhs’
      by (unabbrev_all_tac >>
          rw[] >- intLib.COOPER_TAC >>
          simp[GSYM (PURE_REWRITE_RULE [Once integerTheory.INT_ADD_SYM,integerTheory.INT_1]
                                       integerTheory.int_of_num)]) >>
      simp[] >>    
-     MAP_EVERY qunabbrev_tac [`lhs`,`rhs`] >>
+     MAP_EVERY qunabbrev_tac [‘lhs’,‘rhs’] >>
      simp[store_assign_def,store_v_same_type_def,EL_APPEND_EQN,
           semanticPrimitivesTheory.state_component_equality,LUPDATE_APPEND,
           LUPDATE_def] >>
@@ -197,22 +198,22 @@ val padv_correct = Q.store_thm("padv_correct",`
      simp[DROP_LENGTH_TOO_LONG,LENGTH_LUPDATE] >>
      simp[REWRITE_RULE [ADD1] REPLICATE,LUPDATE_def] >>
      simp[TAKE_LENGTH_TOO_LONG]) >>
-  rpt(qpat_x_assum `do_opapp _ = _` kall_tac) >>
+  rpt(qpat_x_assum ‘do_opapp _ = _’ kall_tac) >>
   ntac 8 (simp[Once evaluate_def]) >>
-  qpat_assum `(LIST_TYPE ^WORD8 --> NUM) LENGTH _` (mp_tac o REWRITE_RULE[ml_translatorTheory.Arrow_def,ml_translatorTheory.AppReturns_def,ml_progTheory.eval_rel_def]) >>
+  qpat_assum ‘(LIST_TYPE ^WORD8 --> NUM) LENGTH _’ (mp_tac o REWRITE_RULE[ml_translatorTheory.Arrow_def,ml_translatorTheory.AppReturns_def,ml_progTheory.eval_rel_def]) >>
   simp[] >> disch_then drule >>
-  qmatch_goalsub_abbrev_tac `refs_fupd (K a1)` >>
-  disch_then(qspec_then `a1` strip_assume_tac) >>
-  qunabbrev_tac `a1` >>
-  Q.REFINE_EXISTS_TAC `extra + 1` >>
+  qmatch_goalsub_abbrev_tac ‘refs_fupd (K a1)’ >>
+  disch_then(qspec_then ‘a1’ strip_assume_tac) >>
+  qunabbrev_tac ‘a1’ >>
+  Q.REFINE_EXISTS_TAC ‘extra + 1’ >>
   simp[dec_clock_def] >>
-  Q.ISPEC_THEN `s2 with refs := s1.refs ++ refs` dxrule evaluate_empty_state_norel >>
+  Q.ISPEC_THEN ‘s2 with refs := s1.refs ++ refs’ dxrule evaluate_empty_state_norel >>
   strip_tac >>
-  qmatch_asmsub_abbrev_tac `clock_fupd (K ack3)` >>
-  Q.REFINE_EXISTS_TAC `extra + ack3` >>
+  qmatch_asmsub_abbrev_tac ‘clock_fupd (K ack3)’ >>
+  Q.REFINE_EXISTS_TAC ‘extra + ack3’ >>
   drule evaluate_add_to_clock >>
-  simp[SimpL ``$==>``] >>
-  disch_then(qspec_then `ack2` mp_tac) >>
+  simp[SimpL “$==>”] >>
+  disch_then(qspec_then ‘ack2’ mp_tac) >>
   strip_tac >>
   dxrule evaluate_add_to_clock >>
   simp[] >>
@@ -220,7 +221,7 @@ val padv_correct = Q.store_thm("padv_correct",`
   fs[NUM_def,INT_def] >>  
   simp[do_app_def] >>
   simp[semanticPrimitivesTheory.opb_lookup_def,lit_same_type_def,Boolv_def,do_if_def] >>
-  Cases_on `LENGTH l < conf.payload_size` >-
+  Cases_on ‘LENGTH l < conf.payload_size’ >-
     (simp[] >>
      ntac 7 (simp[Once evaluate_def]) >>
      simp[do_app_def,store_lookup_def,EL_APPEND_EQN,store_assign_def,
@@ -228,26 +229,26 @@ val padv_correct = Q.store_thm("padv_correct",`
           namespaceTheory.nsOptBind_def,lupdate_append2] >>
      ntac 5 (simp[Once evaluate_def]) >>
      PURE_REWRITE_TAC [ADD_ASSOC] >>
-     qpat_abbrev_tac `ack4 = ack2 + _` >> pop_assum kall_tac >>    
+     qpat_abbrev_tac ‘ack4 = ack2 + _’ >> pop_assum kall_tac >>    
      last_x_assum drule >>
-     qmatch_goalsub_abbrev_tac `refs_fupd (K a1)` >>
-     disch_then(qspec_then `empty_state with refs := a1` mp_tac) >>
+     qmatch_goalsub_abbrev_tac ‘refs_fupd (K a1)’ >>
+     disch_then(qspec_then ‘empty_state with refs := a1’ mp_tac) >>
      simp[] >>
-     qunabbrev_tac `a1` >> strip_tac >>
-     Q.REFINE_EXISTS_TAC `extra + 1` >>
+     qunabbrev_tac ‘a1’ >> strip_tac >>
+     Q.REFINE_EXISTS_TAC ‘extra + 1’ >>
      simp[dec_clock_def] >>
-     Q.ISPEC_THEN `s2 with refs := s1.refs ++ refs` dxrule evaluate_empty_state_norel >>
+     Q.ISPEC_THEN ‘s2 with refs := s1.refs ++ refs’ dxrule evaluate_empty_state_norel >>
      strip_tac >>
-     qmatch_asmsub_abbrev_tac `clock_fupd (K ack5)` >>
-     Q.REFINE_EXISTS_TAC `extra + ack5` >>
+     qmatch_asmsub_abbrev_tac ‘clock_fupd (K ack5)’ >>
+     Q.REFINE_EXISTS_TAC ‘extra + ack5’ >>
      drule evaluate_add_to_clock >>
-     simp[SimpL ``$==>``] >>
-     disch_then(qspec_then `ack4` mp_tac) >>
+     simp[SimpL “$==>”] >>
+     disch_then(qspec_then ‘ack4’ mp_tac) >>
      strip_tac >>
      dxrule evaluate_add_to_clock >>
      simp[] >> disch_then kall_tac >>
      PURE_REWRITE_TAC [ADD_ASSOC] >>
-     qpat_abbrev_tac `ack6 = ack4 + _` >> pop_assum kall_tac >>
+     qpat_abbrev_tac ‘ack6 = ack4 + _’ >> pop_assum kall_tac >>
      simp[evaluate_def,namespaceTheory.nsOptBind_def,ml_progTheory.nsLookup_nsBind_compute,
           do_app_def,store_lookup_def,EL_APPEND_EQN,copy_array_def,integerTheory.INT_ABS,
           LUPDATE_APPEND,LUPDATE_def,opn_lookup_def] >>
@@ -271,13 +272,13 @@ val padv_correct = Q.store_thm("padv_correct",`
           do_app_def,store_lookup_def,EL_APPEND_EQN,copy_array_def,integerTheory.INT_ABS,
           LUPDATE_APPEND,LUPDATE_def,opn_lookup_def,store_assign_def,
           store_v_same_type_def,semanticPrimitivesTheory.state_component_equality] >>
-     `Num (1 + (&conf.payload_size − &LENGTH l)) = 1 + (conf.payload_size - LENGTH l)`
+     ‘Num (1 + (&conf.payload_size − &LENGTH l)) = 1 + (conf.payload_size - LENGTH l)’
        by(intLib.COOPER_TAC) >>
-     `Num (&conf.payload_size − &LENGTH l) = conf.payload_size - LENGTH l`
+     ‘Num (&conf.payload_size − &LENGTH l) = conf.payload_size - LENGTH l’
        by(intLib.COOPER_TAC) >>
      simp[] >>
      simp[REWRITE_RULE [ADD1] REPLICATE,LUPDATE_APPEND,REWRITE_RULE [ADD1] LUPDATE_def] >>
-     `conf.payload_size − LENGTH l = conf.payload_size − (LENGTH l + 1) + 1`
+     ‘conf.payload_size − LENGTH l = conf.payload_size − (LENGTH l + 1) + 1’
        by(intLib.COOPER_TAC) >>
      pop_assum(fn thm => PURE_ONCE_REWRITE_TAC [thm]) >>
      PURE_REWRITE_TAC[REWRITE_RULE [ADD1] LUPDATE_def] >>
@@ -285,7 +286,7 @@ val padv_correct = Q.store_thm("padv_correct",`
      IF_CASES_TAC >- (
         spose_not_then kall_tac >>
         pop_assum mp_tac >> intLib.COOPER_TAC) >>
-     `Num (1 + (&conf.payload_size − &LENGTH l) + &LENGTH l) = conf.payload_size + 1`
+     ‘Num (1 + (&conf.payload_size − &LENGTH l) + &LENGTH l) = conf.payload_size + 1’
        by(intLib.COOPER_TAC) >>
      simp[DROP_LENGTH_TOO_LONG,LENGTH_LUPDATE,LENGTH_REPLICATE] >>
      simp[LUPDATE_REPLICATE,TAKE_APPEND] >>
@@ -293,71 +294,71 @@ val padv_correct = Q.store_thm("padv_correct",`
      simp[pad_def]) >>
     (simp[] >>
      PURE_REWRITE_TAC [ADD_ASSOC] >>
-     qpat_abbrev_tac `ack4 = ack2 + _` >> pop_assum kall_tac >>
+     qpat_abbrev_tac ‘ack4 = ack2 + _’ >> pop_assum kall_tac >>
      ntac 7 (simp[Once evaluate_def]) >>
      simp[do_app_def,store_lookup_def,EL_APPEND_EQN,store_assign_def,
           store_v_same_type_def,ml_progTheory.nsLookup_nsBind_compute,
           namespaceTheory.nsOptBind_def,lupdate_append2] >>
      ntac 10 (simp[Once evaluate_def]) >>
-     qpat_assum `(LIST_TYPE WORD --> NUM --> LIST_TYPE WORD) (combin$C TAKE) _` (mp_tac o REWRITE_RULE[ml_translatorTheory.Arrow_def,ml_translatorTheory.AppReturns_def,ml_progTheory.eval_rel_def]) >>
+     qpat_assum ‘(LIST_TYPE WORD --> NUM --> LIST_TYPE WORD) (combin$C TAKE) _’ (mp_tac o REWRITE_RULE[ml_translatorTheory.Arrow_def,ml_translatorTheory.AppReturns_def,ml_progTheory.eval_rel_def]) >>
      simp[] >> disch_then drule >>
-     qmatch_goalsub_abbrev_tac `refs_fupd (K a1)` >>     
-     disch_then(qspec_then `a1` strip_assume_tac) >>
-     qunabbrev_tac `a1` >>
-     Q.REFINE_EXISTS_TAC `extra + 1` >>
+     qmatch_goalsub_abbrev_tac ‘refs_fupd (K a1)’ >>     
+     disch_then(qspec_then ‘a1’ strip_assume_tac) >>
+     qunabbrev_tac ‘a1’ >>
+     Q.REFINE_EXISTS_TAC ‘extra + 1’ >>
      simp[dec_clock_def] >>
-     Q.ISPEC_THEN `s2 with refs := s1.refs ++ refs` dxrule evaluate_empty_state_norel >>
+     Q.ISPEC_THEN ‘s2 with refs := s1.refs ++ refs’ dxrule evaluate_empty_state_norel >>
      strip_tac >>
-     qmatch_asmsub_abbrev_tac `clock_fupd (K ack5)` >>
-     Q.REFINE_EXISTS_TAC `extra + ack5` >>
+     qmatch_asmsub_abbrev_tac ‘clock_fupd (K ack5)’ >>
+     Q.REFINE_EXISTS_TAC ‘extra + ack5’ >>
      drule evaluate_add_to_clock >>
-     simp[SimpL ``$==>``] >>
-     disch_then(qspec_then `ack4` mp_tac) >>
+     simp[SimpL “$==>”] >>
+     disch_then(qspec_then ‘ack4’ mp_tac) >>
      strip_tac >>
      dxrule evaluate_add_to_clock >>
      simp[] >> disch_then kall_tac >>
-     first_x_assum(qspecl_then [`conf.payload_size`,`Litv (IntLit (&conf.payload_size))`] mp_tac) >>
+     first_x_assum(qspecl_then [‘conf.payload_size’,‘Litv (IntLit (&conf.payload_size))’] mp_tac) >>
      impl_tac >- simp[NUM_def,INT_def] >>
-     qmatch_goalsub_abbrev_tac `refs_fupd (K a1)` >>
-     disch_then(qspec_then `a1` strip_assume_tac) >>
-     qunabbrev_tac `a1` >>
-     Q.REFINE_EXISTS_TAC `extra + 1` >>
+     qmatch_goalsub_abbrev_tac ‘refs_fupd (K a1)’ >>
+     disch_then(qspec_then ‘a1’ strip_assume_tac) >>
+     qunabbrev_tac ‘a1’ >>
+     Q.REFINE_EXISTS_TAC ‘extra + 1’ >>
      simp[dec_clock_def] >>
      PURE_REWRITE_TAC [ADD_ASSOC] >>
-     qpat_abbrev_tac `ack6 = ack4 + _` >> pop_assum kall_tac >>
-     Q.ISPEC_THEN `s2 with refs := s1.refs ++ refs` dxrule evaluate_empty_state_norel >>
+     qpat_abbrev_tac ‘ack6 = ack4 + _’ >> pop_assum kall_tac >>
+     Q.ISPEC_THEN ‘s2 with refs := s1.refs ++ refs’ dxrule evaluate_empty_state_norel >>
      strip_tac >>
-     qmatch_asmsub_abbrev_tac `clock_fupd (K ack7)` >>
-     Q.REFINE_EXISTS_TAC `extra + ack7` >>
+     qmatch_asmsub_abbrev_tac ‘clock_fupd (K ack7)’ >>
+     Q.REFINE_EXISTS_TAC ‘extra + ack7’ >>
      drule evaluate_add_to_clock >>
-     simp[SimpL ``$==>``] >>
-     disch_then(qspec_then `ack6` mp_tac) >>
+     simp[SimpL “$==>”] >>
+     disch_then(qspec_then ‘ack6’ mp_tac) >>
      strip_tac >>
      dxrule evaluate_add_to_clock >>
      simp[] >>
      disch_then kall_tac >>
      PURE_REWRITE_TAC [ADD_ASSOC] >>
-     qpat_abbrev_tac `ack8 = ack6 + _` >> pop_assum kall_tac >>
+     qpat_abbrev_tac ‘ack8 = ack6 + _’ >> pop_assum kall_tac >>
      simp[Once evaluate_def] >>
      last_x_assum drule >>
-     qmatch_goalsub_abbrev_tac `refs_fupd (K a1)` >>
-     disch_then(qspec_then `empty_state with refs := a1` mp_tac) >>
+     qmatch_goalsub_abbrev_tac ‘refs_fupd (K a1)’ >>
+     disch_then(qspec_then ‘empty_state with refs := a1’ mp_tac) >>
      simp[] >>
-     qunabbrev_tac `a1` >> strip_tac >>
-     Q.REFINE_EXISTS_TAC `extra + 1` >>
+     qunabbrev_tac ‘a1’ >> strip_tac >>
+     Q.REFINE_EXISTS_TAC ‘extra + 1’ >>
      simp[dec_clock_def] >>
-     Q.ISPEC_THEN `s2 with refs := s1.refs ++ refs` dxrule evaluate_empty_state_norel >>
+     Q.ISPEC_THEN ‘s2 with refs := s1.refs ++ refs’ dxrule evaluate_empty_state_norel >>
      strip_tac >>
-     qmatch_asmsub_abbrev_tac `clock_fupd (K ack9)` >>
-     Q.REFINE_EXISTS_TAC `extra + ack9` >>
+     qmatch_asmsub_abbrev_tac ‘clock_fupd (K ack9)’ >>
+     Q.REFINE_EXISTS_TAC ‘extra + ack9’ >>
      drule evaluate_add_to_clock >>
-     simp[SimpL ``$==>``] >>
-     disch_then(qspec_then `ack8` mp_tac) >>
+     simp[SimpL “$==>”] >>
+     disch_then(qspec_then ‘ack8’ mp_tac) >>
      strip_tac >>
      dxrule evaluate_add_to_clock >>
      simp[] >> disch_then kall_tac >>
      PURE_REWRITE_TAC [ADD_ASSOC] >>
-     qpat_abbrev_tac `ack10 = ack8 + _` >> pop_assum kall_tac >>
+     qpat_abbrev_tac ‘ack10 = ack8 + _’ >> pop_assum kall_tac >>
      simp[evaluate_def,namespaceTheory.nsOptBind_def,ml_progTheory.nsLookup_nsBind_compute,
           do_app_def,store_lookup_def,EL_APPEND_EQN,copy_array_def,integerTheory.INT_ABS,
           LUPDATE_APPEND,LUPDATE_def] >>
@@ -366,43 +367,44 @@ val padv_correct = Q.store_thm("padv_correct",`
      simp[store_assign_def,store_v_same_type_def,EL_APPEND_EQN,
           semanticPrimitivesTheory.state_component_equality,LUPDATE_APPEND,
           REWRITE_RULE [ADD1] REPLICATE,LUPDATE_def,TAKE_TAKE] >>
-     rw[pad_def,DROP_NIL] >> intLib.COOPER_TAC));
+     rw[pad_def,DROP_NIL] >> intLib.COOPER_TAC)
+  );
 
-val ffi_accepts_rel_def = Define `
+val ffi_accepts_rel_def = Define ‘
   ffi_accepts_rel stpred pred oracle =
-  !st s conf bytes.
-    stpred st.ffi_state /\ st.oracle = oracle /\ pred s conf bytes ==>
-    ?ffi. st.oracle s st.ffi_state conf bytes = Oracle_return ffi bytes /\
-          stpred ffi`
+  ∀st s conf bytes.
+    stpred st.ffi_state ∧ st.oracle = oracle ∧ pred s conf bytes ⇒
+    ∃ffi. st.oracle s st.ffi_state conf bytes = Oracle_return ffi bytes ∧
+          stpred ffi’;
 
-val send_events_def = Define `
+val send_events_def = Define ‘
   send_events conf dest d =
-  MAP (λm. IO_event "send" dest (ZIP (m,m)))(compile_message conf d)`
+  MAP (λm. IO_event "send" dest (ZIP (m,m)))(compile_message conf d)’;
 
-val update_state_def = Define `
-  (update_state st oracle [] = st) /\
+val update_state_def = Define ‘
+  (update_state st oracle [] = st) ∧
   (update_state st oracle (IO_event s c b::es) =
    update_state (@st'. oracle s st c (MAP FST b) = Oracle_return st' (MAP SND b))
-                oracle es)`
+                oracle es)’;
 
 val LUPDATE_SAME' = Q.prove(
-  `n < LENGTH ls /\ EL n ls = a ==> LUPDATE a n ls = ls`,
+  ‘n < LENGTH ls ∧ EL n ls = a ⇒ LUPDATE a n ls = ls’,
   metis_tac[LUPDATE_SAME]);
 
-val sendloop_correct = Q.store_thm("sendloop_correct",`
-  !conf l env env' lv le s refs stpred dest.
-  env_asm env' conf /\
-  conf.payload_size <> 0 /\
-  LIST_TYPE ^WORD8 l lv /\
-  nsLookup env.v (Short "sendloop") = SOME(Recclosure env' (sendloop conf (MAP (CHR o w2n) dest)) "sendloop") /\
-  nsLookup env.v (Short "x") = SOME lv /\
-  stpred s.ffi.ffi_state /\
+Theorem sendloop_correct
+ ‘∀conf l env env' lv le s refs stpred dest.
+  env_asm env' conf ∧
+  conf.payload_size ≠ 0 ∧
+  LIST_TYPE ^WORD8 l lv ∧
+  nsLookup env.v (Short "sendloop") = SOME(Recclosure env' (sendloop conf (MAP (CHR o w2n) dest)) "sendloop") ∧
+  nsLookup env.v (Short "x") = SOME lv ∧
+  stpred s.ffi.ffi_state ∧
   ffi_accepts_rel
     stpred
-    (λs c bytes. s = "send" /\ c = dest /\ LENGTH bytes = SUC conf.payload_size)
+    (λs c bytes. s = "send" ∧ c = dest ∧ LENGTH bytes = SUC conf.payload_size)
     s.ffi.oracle
-  ==>
-  ?ck1 ck2 refs' num lv'.
+  ⇒
+  ∃ck1 ck2 refs' num lv'.
   evaluate$evaluate (s with clock:= ck1) env [App Opapp [Var (Short "sendloop"); Var(Short "x")]] =
                     (s with
                        <|clock := ck2; refs := APPEND s.refs refs';
@@ -410,34 +412,34 @@ val sendloop_correct = Q.store_thm("sendloop_correct",`
                          <|io_events := s.ffi.io_events ++ send_events conf dest l;
                            ffi_state := update_state s.ffi.ffi_state s.ffi.oracle (send_events conf dest l)
                           |>
-                        |>, Rval [Conv NONE []])
-  `,
-  ho_match_mp_tac compile_message_ind >> rpt strip_tac >>
+                        |>, Rval [Conv NONE []])’
+ (ho_match_mp_tac compile_message_ind>>
+  rpt strip_tac >>
   ntac 4 (simp[Once evaluate_def]) >>
   simp[do_opapp_def] >>
   ntac 2 (simp[Once sendloop_def]) >>
   simp[find_recfun_def] >>
-  Q.REFINE_EXISTS_TAC `extra + 1` >>
+  Q.REFINE_EXISTS_TAC ‘extra + 1’ >>
   simp[dec_clock_def] >>
   simp[Once evaluate_def] >>
-  qmatch_goalsub_abbrev_tac `evaluate _ env1` >>
-  `env_asm env1 conf`
-    by fs[Abbr `env1`,env_asm_def,build_rec_env_def,sendloop_def,has_v_def,in_module_def] >>
+  qmatch_goalsub_abbrev_tac ‘evaluate _ env1’ >>
+  ‘env_asm env1 conf’
+    by fs[Abbr ‘env1’,env_asm_def,build_rec_env_def,sendloop_def,has_v_def,in_module_def] >>
   drule(INST_TYPE [alpha |-> beta] padv_correct) >> disch_then drule >>
-  disch_then(qspecl_then [`Var(Short "x")`,`s`,`s`,`[]`] mp_tac) >>
-  impl_tac >- simp[evaluate_def,Abbr `env1`,semanticPrimitivesTheory.state_component_equality] >>
+  disch_then(qspecl_then [‘Var(Short "x")’,‘s’,‘s’,‘[]’] mp_tac) >>
+  impl_tac >- simp[evaluate_def,Abbr ‘env1’,semanticPrimitivesTheory.state_component_equality] >>
   strip_tac >>
-  qmatch_asmsub_abbrev_tac `clock_fupd (K ack1)` >>
-  Q.REFINE_EXISTS_TAC `extra + ack1` >>
+  qmatch_asmsub_abbrev_tac ‘clock_fupd (K ack1)’ >>
+  Q.REFINE_EXISTS_TAC ‘extra + ack1’ >>
   dxrule evaluate_add_to_clock >>
   simp[] >> disch_then kall_tac >>
   ntac 4 (simp[Once evaluate_def]) >>  
   simp[ml_progTheory.nsLookup_nsBind_compute,namespaceTheory.nsOptBind_def,
        do_app_def,ffiTheory.call_FFI_def] >>
   simp[Once evaluate_def] >>
-  qhdtm_assum `ffi_accepts_rel` (mp_tac o REWRITE_RULE [ffi_accepts_rel_def]) >>
+  qhdtm_assum ‘ffi_accepts_rel’ (mp_tac o REWRITE_RULE [ffi_accepts_rel_def]) >>
   disch_then drule >> simp[] >>
-  disch_then(qspec_then `pad conf l` mp_tac) >>
+  disch_then(qspec_then ‘pad conf l’ mp_tac) >>
   impl_keep_tac >- rw[pad_def] >>
   strip_tac >>
   simp[IMPLODE_EXPLODE_I,MAP_MAP_o,o_DEF,
@@ -448,36 +450,36 @@ val sendloop_correct = Q.store_thm("sendloop_correct",`
   ntac 8 (simp[Once evaluate_def]) >>
   simp[do_app_def,ml_progTheory.nsLookup_nsBind_compute,
        namespaceTheory.nsOptBind_def] >>
-  qmatch_goalsub_abbrev_tac `evaluate _ env2` >>
-  `env_asm env2 conf`
-    by fs[Abbr `env2`,env_asm_def,build_rec_env_def,sendloop_def,has_v_def,in_module_def] >>
+  qmatch_goalsub_abbrev_tac ‘evaluate _ env2’ >>
+  ‘env_asm env2 conf’
+    by fs[Abbr ‘env2’,env_asm_def,build_rec_env_def,sendloop_def,has_v_def,in_module_def] >>
   first_assum (strip_assume_tac o REWRITE_RULE[env_asm_def]) >>
-  qunabbrev_tac `env2` >>
+  qunabbrev_tac ‘env2’ >>
   fs[has_v_def] >>
-  qpat_assum `(LIST_TYPE ^WORD8 --> NUM) LENGTH _` (mp_tac o REWRITE_RULE[ml_translatorTheory.Arrow_def,ml_translatorTheory.AppReturns_def,ml_progTheory.eval_rel_def]) >>
+  qpat_assum ‘(LIST_TYPE ^WORD8 --> NUM) LENGTH _’ (mp_tac o REWRITE_RULE[ml_translatorTheory.Arrow_def,ml_translatorTheory.AppReturns_def,ml_progTheory.eval_rel_def]) >>
   simp[] >> disch_then drule >>
-  qmatch_goalsub_abbrev_tac `refs_fupd (K a1)` >>
-  disch_then(qspec_then `a1` strip_assume_tac) >>
-  qunabbrev_tac `a1` >>
-  Q.REFINE_EXISTS_TAC `extra + 1` >>
+  qmatch_goalsub_abbrev_tac ‘refs_fupd (K a1)’ >>
+  disch_then(qspec_then ‘a1’ strip_assume_tac) >>
+  qunabbrev_tac ‘a1’ >>
+  Q.REFINE_EXISTS_TAC ‘extra + 1’ >>
   simp[dec_clock_def] >>
-    qmatch_goalsub_abbrev_tac `ffi_fupd (K a1)` >>
-  Q.ISPEC_THEN `s with ffi := a1` dxrule evaluate_empty_state_norel >>
-  qunabbrev_tac `a1` >>
+    qmatch_goalsub_abbrev_tac ‘ffi_fupd (K a1)’ >>
+  Q.ISPEC_THEN ‘s with ffi := a1’ dxrule evaluate_empty_state_norel >>
+  qunabbrev_tac ‘a1’ >>
   strip_tac >>
-  rename1 `ack2 + _` >>
-  qmatch_asmsub_abbrev_tac `clock_fupd (K ack3)` >>
-  Q.REFINE_EXISTS_TAC `extra + ack3` >>
+  rename1 ‘ack2 + _’ >>
+  qmatch_asmsub_abbrev_tac ‘clock_fupd (K ack3)’ >>
+  Q.REFINE_EXISTS_TAC ‘extra + ack3’ >>
   dxrule evaluate_add_to_clock >>
-  simp[SimpL ``$==>``] >>
-  disch_then(qspec_then `ack2` mp_tac) >>
+  simp[SimpL “$==>”] >>
+  disch_then(qspec_then ‘ack2’ mp_tac) >>
   strip_tac >>
   dxrule evaluate_add_to_clock >>
   simp[] >>
   disch_then kall_tac >>
   fs[NUM_def,INT_def] >>
   PURE_REWRITE_TAC [ADD_ASSOC] >>
-  qpat_abbrev_tac `ack4 = ack2 + _` >> pop_assum kall_tac >>
+  qpat_abbrev_tac ‘ack4 = ack2 + _’ >> pop_assum kall_tac >>
   simp[do_if_def,opb_lookup_def] >>
   IF_CASES_TAC >- (* base case of induction: LENGTH l <= conf.payload_size *)
     (simp[Once evaluate_def,do_con_check_def,build_conv_def,semanticPrimitivesTheory.state_component_equality,ffiTheory.ffi_state_component_equality] >>
@@ -487,73 +489,74 @@ val sendloop_correct = Q.store_thm("sendloop_correct",`
   (* Inductive case: L *)
   simp[] >>
   ntac 8 (simp[Once evaluate_def]) >>
-  qpat_assum `(LIST_TYPE WORD --> NUM --> LIST_TYPE WORD) (combin$C DROP) _` (mp_tac o REWRITE_RULE[ml_translatorTheory.Arrow_def,ml_translatorTheory.AppReturns_def,ml_progTheory.eval_rel_def]) >>
+  qpat_assum ‘(LIST_TYPE WORD --> NUM --> LIST_TYPE WORD) (combin$C DROP) _’ (mp_tac o REWRITE_RULE[ml_translatorTheory.Arrow_def,ml_translatorTheory.AppReturns_def,ml_progTheory.eval_rel_def]) >>
   simp[] >> disch_then drule >>
-  qmatch_goalsub_abbrev_tac `refs_fupd (K a1)` >>     
-  disch_then(qspec_then `a1` strip_assume_tac) >>
-  qunabbrev_tac `a1` >>
-  Q.REFINE_EXISTS_TAC `extra + 1` >>
+  qmatch_goalsub_abbrev_tac ‘refs_fupd (K a1)’ >>     
+  disch_then(qspec_then ‘a1’ strip_assume_tac) >>
+  qunabbrev_tac ‘a1’ >>
+  Q.REFINE_EXISTS_TAC ‘extra + 1’ >>
   simp[dec_clock_def] >>
-  qmatch_goalsub_abbrev_tac `ffi_fupd (K a1)` >>
-  Q.ISPEC_THEN `s with ffi := a1` dxrule evaluate_empty_state_norel >>
-  qunabbrev_tac `a1` >>
+  qmatch_goalsub_abbrev_tac ‘ffi_fupd (K a1)’ >>
+  Q.ISPEC_THEN ‘s with ffi := a1’ dxrule evaluate_empty_state_norel >>
+  qunabbrev_tac ‘a1’ >>
   strip_tac >>  
-  qmatch_asmsub_abbrev_tac `clock_fupd (K ack5)` >>
-  Q.REFINE_EXISTS_TAC `extra + ack5` >>
+  qmatch_asmsub_abbrev_tac ‘clock_fupd (K ack5)’ >>
+  Q.REFINE_EXISTS_TAC ‘extra + ack5’ >>
   dxrule evaluate_add_to_clock >>
-  simp[SimpL ``$==>``] >>
-  disch_then(qspec_then `ack4` mp_tac) >>
+  simp[SimpL “$==>”] >>
+  disch_then(qspec_then ‘ack4’ mp_tac) >>
   strip_tac >>
   dxrule evaluate_add_to_clock >>
   simp[] >> disch_then kall_tac >>
-  first_x_assum(qspecl_then [`conf.payload_size`,`Litv (IntLit (&conf.payload_size))`] mp_tac) >>
+  first_x_assum(qspecl_then [‘conf.payload_size’,‘Litv (IntLit (&conf.payload_size))’] mp_tac) >>
   impl_tac >- simp[NUM_def,INT_def] >>
-  qmatch_goalsub_abbrev_tac `refs_fupd (K a1)` >>
-  disch_then(qspec_then `a1` strip_assume_tac) >>
-  qunabbrev_tac `a1` >>
-  qmatch_goalsub_abbrev_tac `ffi_fupd (K a1)` >>
-  Q.ISPEC_THEN `s with ffi := a1` dxrule evaluate_empty_state_norel >>
-  qunabbrev_tac `a1` >>
+  qmatch_goalsub_abbrev_tac ‘refs_fupd (K a1)’ >>
+  disch_then(qspec_then ‘a1’ strip_assume_tac) >>
+  qunabbrev_tac ‘a1’ >>
+  qmatch_goalsub_abbrev_tac ‘ffi_fupd (K a1)’ >>
+  Q.ISPEC_THEN ‘s with ffi := a1’ dxrule evaluate_empty_state_norel >>
+  qunabbrev_tac ‘a1’ >>
   strip_tac >>
-  Q.REFINE_EXISTS_TAC `extra + 1` >>
+  Q.REFINE_EXISTS_TAC ‘extra + 1’ >>
   simp[dec_clock_def] >>
   PURE_REWRITE_TAC [ADD_ASSOC] >>
-  qpat_abbrev_tac `ack6 = ack4 + _` >> pop_assum kall_tac >>
-  qmatch_asmsub_abbrev_tac `clock_fupd (K ack7)` >>
-  Q.REFINE_EXISTS_TAC `extra + ack7` >>
+  qpat_abbrev_tac ‘ack6 = ack4 + _’ >> pop_assum kall_tac >>
+  qmatch_asmsub_abbrev_tac ‘clock_fupd (K ack7)’ >>
+  Q.REFINE_EXISTS_TAC ‘extra + ack7’ >>
   dxrule evaluate_add_to_clock >>
-  simp[SimpL ``$==>``] >>
-  disch_then(qspec_then `ack6` mp_tac) >>
+  simp[SimpL “$==>”] >>
+  disch_then(qspec_then ‘ack6’ mp_tac) >>
   strip_tac >>
   dxrule evaluate_add_to_clock >>
   simp[] >>
   disch_then kall_tac >>
   PURE_REWRITE_TAC [ADD_ASSOC] >>
-  qpat_abbrev_tac `ack8 = ack6 + _` >> pop_assum kall_tac >>
+  qpat_abbrev_tac ‘ack8 = ack6 + _’ >> pop_assum kall_tac >>
   fs[send_events_def,final_pad_LENGTH] >>
-  qmatch_goalsub_abbrev_tac `evaluate _ env2` >>  
-  qpat_x_assum `env_asm env' conf` assume_tac >>
+  qmatch_goalsub_abbrev_tac ‘evaluate _ env2’ >>  
+  qpat_x_assum ‘env_asm env' conf’ assume_tac >>
   last_x_assum drule >> disch_then drule >>
-  disch_then(qspec_then `env2` mp_tac) >>
-  qmatch_goalsub_abbrev_tac `ffi_fupd (K a1)` >>
-  qmatch_goalsub_abbrev_tac `refs_fupd (K a2)` >>
-  disch_then(qspec_then `s with <|ffi := a1; refs := a2 |>` mp_tac) >>
-  disch_then(qspecl_then [`stpred`,`dest`] mp_tac) >>
-  qunabbrev_tac `a1` >> qunabbrev_tac `a2` >>
+  disch_then(qspec_then ‘env2’ mp_tac) >>
+  qmatch_goalsub_abbrev_tac ‘ffi_fupd (K a1)’ >>
+  qmatch_goalsub_abbrev_tac ‘refs_fupd (K a2)’ >>
+  disch_then(qspec_then ‘s with <|ffi := a1; refs := a2 |>’ mp_tac) >>
+  disch_then(qspecl_then [‘stpred’,‘dest’] mp_tac) >>
+  qunabbrev_tac ‘a1’ >> qunabbrev_tac ‘a2’ >>
   impl_tac >-
     (unabbrev_all_tac >>
      simp[sendloop_def,build_rec_env_def,o_DEF,namespaceTheory.nsOptBind_def]) >>
   simp[] >> strip_tac >>
-  qmatch_asmsub_abbrev_tac `clock_fupd (K ack9)` >>
-  Q.REFINE_EXISTS_TAC `extra + ack9` >>
+  qmatch_asmsub_abbrev_tac ‘clock_fupd (K ack9)’ >>
+  Q.REFINE_EXISTS_TAC ‘extra + ack9’ >>
   dxrule evaluate_add_to_clock >>
-  simp[SimpL ``$==>``] >>
-  disch_then(qspec_then `ack8` mp_tac) >>
+  simp[SimpL “$==>”] >>
+  disch_then(qspec_then ‘ack8’ mp_tac) >>
   strip_tac >>
   dxrule evaluate_add_to_clock >>
   simp[] >> disch_then kall_tac >>
   simp[semanticPrimitivesTheory.state_component_equality,ffiTheory.ffi_state_component_equality] >>
   conj_tac >> CONV_TAC(RHS_CONV(PURE_ONCE_REWRITE_CONV [compile_message_def])) >>
-  simp[final_pad_LENGTH,update_state_def]);
+  simp[final_pad_LENGTH,update_state_def]
+  );
 
 val _ = export_theory ();
